src/examples/memstuff.v
@@ -1,0 +1,94 @@
+Require Import Ssreflect.ssreflect Ssreflect.ssrbool Ssreflect.ssrnat Ssreflect.eqtype Ssreflect.seq Ssreflect.fintype.
+Require Import x86proved.x86.procstate x86proved.x86.procstatemonad x86proved.bitsops x86proved.bitsprops x86proved.bitsopsprops.
+Require Import x86proved.spred x86proved.septac x86proved.spec x86proved.spectac x86proved.x86.basic x86proved.x86.basicprog x86proved.x86.program.
+Require Import x86proved.x86.instr x86proved.x86.instrsyntax x86proved.x86.instrcodec x86proved.x86.instrrules x86proved.reader x86proved.pointsto x86proved.cursor x86proved.x86.basic x86proved.x86.macros x86proved.charge.ilogic.
+
+Set Implicit Arguments.
+Unset Strict Implicit.
+Import Prenex Implicits.
+
+Open Scope instr_scope.
+
+Definition splits (p q r: DWORD) (vs ws: seq DWORD) :=
+  p -- q :-> vs ** q -- r :-> ws.
+
+Definition nextCode := (ADD ESI, 4). 
+Definition nextSpec code := 
+  Forall (p q r: DWORD), Forall vs w ws, 
+  basic (splits p q r vs (w::ws) ** ESI ~= q) code empOP
+        (splits p (q+#4) r (vs++[::w]) ws ** ESI ~= (q+#4)) @ OSZCP?.
+
+Lemma nextCorrect : |-- nextSpec nextCode. 
+Proof. rewrite /nextSpec/nextCode. specintros => *. autorewrite with push_at.
+basic apply *.
+rewrite /splits. 
+rewrite -> (seqFixedMemIsCons' _). rewrite seqMemIsCat pairMemIsPair'. sbazooka. 
+rewrite -> seqMemIsCons. sbazooka. 
+rewrite -> seqMemIsNil. sbazooka. 
+Qed. 
+
+Definition opSizeToNat s := match s with OpSize1 => 1 | OpSize2 => 2 | OpSize4 => 4 end.
+
+Lemma MOV_RM0aux_rule s (r1: VReg s) (r2:Reg)  (pd:DWORD) (v1 v2: VWORD s) :
+  |-- basic (r1 ~= v1 ** r2 ~= pd ** pd -- (pd+#opSizeToNat s) :-> v2)
+            (MOV r1, [r2]) empOP
+            (r1 ~= v2 ** r2 ~= pd ** pd -- (pd+#opSizeToNat s) :-> v2).
+Proof. rewrite ->memIsLe at 1. specintros => LE. rewrite ->memIs_pointsTo at 1.
+destruct s; basic apply *; rewrite -> (fixedMemIs_pointsTo (n:=_)) => //; reflexivity. 
+Qed.
+
+Global Instance: forall s (r1: VReg s) (r2: Reg), instrrule (MOV r1, [r2]) := @MOV_RM0aux_rule.
+
+Lemma MOV_M0Raux_rule s (r1: VReg s) (r2:Reg)  (pd:DWORD) (v1 v2: VWORD s) :
+  |-- basic (r1 ~= v1 ** r2 ~= pd ** pd -- (pd+#opSizeToNat s) :-> v2)
+            (MOV [r2], r1) empOP
+            (r1 ~= v1 ** r2 ~= pd ** pd -- (pd+#opSizeToNat s) :-> v1).
+Proof. rewrite -> memIsLe at 1. specintros => LE. rewrite -> memIs_pointsTo at 1. 
+destruct s; basic apply *; rewrite -> (fixedMemIs_pointsTo (n:=_)) => //; reflexivity. 
+Qed.
+Global Instance: forall s (r1: VReg s) (r2: Reg), instrrule (MOV [r2], r1) := @MOV_M0Raux_rule.
+
+Definition getCode (dst:Reg):program := (MOV dst, [ESI]). 
+Definition getSpec (dst:Reg) code :=   
+  Forall (p q r: DWORD), Forall vs w ws oldv, 
+  basic 
+  (dst ~= oldv)
+  code 
+  empOP
+  (dst ~= w) @ (splits p q r vs (w::ws) ** ESI ~= q).
+
+Hint Unfold readVWORD opSizeToNat : instrrules_all.
+
+Lemma getCorrect (dst: Reg):
+  |-- getSpec dst (getCode dst). 
+Proof.
+rewrite /getSpec/getCode. specintros => p q r vs w ws oldv. autorewrite with push_at.
+rewrite /splits. rewrite -> (seqFixedMemIsCons' _).
+basic apply (MOV_RM0aux_rule (s:=OpSize4)). 
+Qed. 
+
+Lemma putCorrect (p q r: DWORD) vs w ws oldv :
+  |-- basic 
+  (splits p q r vs (oldv::ws) ** ESI ~= q ** EAX ~= w)
+  (MOV [ESI], EAX)
+  empOP
+  (splits p q r vs (w::ws) ** ESI ~= q ** EAX ~= w).
+Proof.
+rewrite /splits. do 2 rewrite -> (seqFixedMemIsCons' _).
+basic apply (MOV_M0Raux_rule (s:=OpSize4)). 
+Qed. 
+
+Lemma atEndCorrect (p q r: DWORD) (vs ws: seq DWORD):
+  |-- basic
+  (splits p q r vs ws ** ESI ~= q ** ZF? ** OF? ** SF? ** CF? ** PF?)
+  (CMP ESI, r)
+  empOP
+  (splits p q r vs ws ** ESI ~= q ** ZF ~= (if ws is nil then true else false) ** OF? ** SF? ** CF? ** PF?).
+Proof. rewrite /splits. destruct ws. 
+- rewrite seqMemIsNil. 
+  specintros => [[->]]. basicCMP_ZC. 
+- rewrite -> (seqFixedMemIsConsNE (n:=4)) at 1 => //.  
+  specintros =>/negbTE <-. basicCMP_ZC. 
+  (* Why doesn't it pick this up automatically? *) apply FixedMemIsDWORD. 
+Qed. 
+
