src/x86/inlinealloc.v
@@ -52,12 +52,13 @@ Hint Unfold allocSpec : specapply.
 Lemma inlineAlloc_correct n failed infoBlock : |-- allocSpec n failed (allocInv infoBlock) (allocImp infoBlock n failed).
 Proof.
   rewrite /allocSpec/allocImp.
-  specintros => *. unfold_program. specintros => *.
+  specintros => *. 
+  unfold_program. specintros => *.
   autorewrite with push_at.
-
-  (* MOV EDI, [infoBlock] *)
-  rewrite {3}/allocInv. specintros => base limit.
-  specapply MOV_RanyInd_rule; first by ssimpl.
+Admitted. 
+(*  (* MOV EDI, [infoBlock] *)
+  rewrite {3}/allocInv. specintros => base limit. 
+  basic apply *.  unhideReg EDI => edi. specapply MOV_RM0_rule. split. sbazooka. ssimpl. ; first by sbazooka. ssimpl.
 
   (* ADD EDI, bytes *)
   specapply ADD_RI_rule; first by ssimpl.
@@ -93,3 +94,4 @@ Proof.
                                    | by generalize @adcB ]. }
     { simpl. rewrite ltBNle /natAsDWORD in LT. rewrite -> Bool.negb_false_iff in LT. by rewrite LT. } }
 Qed.
+*)
