src/x86/instrrules/or.v
@@ -2,23 +2,20 @@
 Require Import x86proved.x86.instrrules.core.
 Import x86.instrrules.core.instrruleconfig.
 
-Lemma OR_RM_rule (pd:DWORD) (r1:Reg) (r2:Reg) (v1 v2:DWORD) (offset:nat) (v:DWORD) :
+Lemma OR_RM_rule s (pd:DWORD) (r1:VReg s) (r2:Reg) (v1 v2:VWORD s) (offset:nat) (v:VWORD s) :
   orB v1 v2 = v ->
   |-- basic (r1 ~= v1 ** r2 ~= pd ** pd +# offset :-> v2 ** OSZCP?)
             (OR r1, [r2 + offset]) empOP
             (r1 ~= v ** r2 ~= pd ** pd +# offset :-> v2 **
              OSZCP false (msb v) (v == #0) false (lsb v)).
-Proof. move => ?; subst. 
-change (stateIs r1) with (@VRegIs OpSize4 r1). 
-do_instrrule_triple. 
-Qed.
+Proof. move => ?; subst. destruct s; do_instrrule_triple. Qed.
 
 (** We make this rule an instance of the typeclass, and leave
     unfolding things like [specAtDstSrc] to the getter tactic
     [get_instrrule_of]. *)
-Instance: forall (r1 r2 : Reg) (offset : nat), instrrule (OR r1, [r2 + offset]) := fun r1 r2 offset pd v1 v2 => @OR_RM_rule pd r1 r2 v1 v2 offset _ (refl_equal _).
+Instance: forall s (r1:VReg s) (r2 : Reg) (offset : nat), instrrule (OR r1, [r2 + offset]) := fun s (r1:VReg s) r2 offset pd v1 v2 => @OR_RM_rule s pd r1 r2 v1 v2 offset _ (refl_equal _).
 
-Corollary OR_RM_ruleNoFlags (pd:DWORD) (r1 r2:Reg) v1 (v2:DWORD) (offset:nat):
+Corollary OR_RM_ruleNoFlags s (pd:DWORD) (r1:VReg s) (r2:Reg) (v1 v2:VWORD s) (offset:nat):
   |-- basic (r1~=v1) (OR r1, [r2 + offset]) empOP (r1~=orB v1 v2)
              @ (r2 ~= pd ** pd +# offset :-> v2 ** OSZCP?).
 Proof. autorewrite with push_at. basic apply *. Qed.
